upd

coq-formalisations/FullProduct/FullProduct.v
@@ -13,70 +13,171 @@ Definition ident := positive.
 Open Scope Z_scope.
 
 
-
-
+Arguments ok_lvalue [ops].
+Arguments ok_expr [ops].
+Arguments okSC_lvalue [ops].
+Arguments okSC_expr [ops].
+ 
 Section FullProductTrf.
 
 Variable ops: opSig.
 
-Variable lFun : LeakFun ops.
+Definition ok_upd (e: expr ops) : cmd ops :=
+ Assign ok_lvalue (And ok_expr e).
 
-Parameter assertEqLeak : expr ops -> cmd ops.
-Parameter assertEqExpr : expr ops -> cmd ops.
-Parameter ok_get : expr ops.
-Parameter okSC_get : expr ops.
-Parameter ok_reg : expr ops -> cmd ops.
+Variable lspec: LeakSpec ops.
+
+Definition EqLeak (e1 e2: expr ops): expr ops :=
+ EqSeqExpr (preleak lspec e1) (preleak lspec e2).
+
+Lemma isTrue_EqLeak: forall st st1 st2 e,
+ isTrue_expr (joinState (st1,st2,st)) (EqLeak (expr_i1 e) (expr_i2 e))
+ <-> leak_expr (preleak lspec) st1 e = leak_expr (preleak lspec) st2 e.
+Proof.
+admit (*
+move=> st1 st2 e;
+rewrite isTrue_EqSeqExpr /leak_expr !preleak_ren -map_comp.
+have ->:[seq eval_expr (joinState st1 st2) (ren_expr id_i1 x)
+        | x <- preleak lspec e] = [seq eval_expr st1 x | x <- preleak lspec e].
+ by apply eq_map => x; rewrite eval_expr_join_i1.
+rewrite -map_comp.
+have ->:[seq eval_expr (joinState st1 st2) (ren_expr id_i2 x)
+        | x <- preleak lspec e] = [seq eval_expr st2 x | x <- preleak lspec e].
+ by apply eq_map => x; rewrite eval_expr_join_i2.
+have ->: [seq inr (eval_expr st1 e0) | e0 <- preleak lspec e] =
+         map (@inr bool Z) [seq eval_expr st1 x | x <- preleak lspec e] .
+ by rewrite map_comp.
+have ->: [seq inr (eval_expr st2 e0) | e0 <- preleak lspec e] =
+         map (@inr bool Z) [seq eval_expr st2 x | x <- preleak lspec e] .
+ by rewrite map_comp.
+split => H; first by rewrite H.
+have inr_inj: injective (@inr bool Z) by move=> x1 x2 [->].
+by apply (inj_map inr_inj).
+*).
+Qed.
+
+Definition assertEqLeak (e: expr ops): cmd ops :=
+ Assert (EqLeak (ren_expr false e) (ren_expr true e)).
+Definition assertEqLeakTest (e: expr ops): cmd ops :=
+ Assert (And (Equal (IsTrue (ren_expr false e)) (IsTrue (ren_expr true e)))
+             (EqLeak (ren_expr false e) (ren_expr true e))).
+
 
 Fixpoint productTrf (c: cmd ops) {struct c} : cmd ops :=
  match c with
  | Skip => @Skip ops
- | Assert e => Seq (Assert (expr_i false e)) (Assert (expr_i true e))
- | Assume e => Seq (Assume (expr_i false e)) (Assume (expr_i true e))
+ | Assert e => Seq (Assert (ren_expr false e)) (Assert (ren_expr true e))
+ | Assume e => Seq (Assume (ren_expr false e)) (Assume (ren_expr true e))
  | Assign x e => Seq (Seq (assertEqLeak (ValOf x))
                           (assertEqLeak e))
-                     (Seq (Assign (lvalue_i false x) (expr_i false e))
-                          (Assign (lvalue_i true x) (expr_i true e)))
+                     (Seq (Assign (ren_lvalue false x) (ren_expr false e))
+                          (Assign (ren_lvalue true x) (ren_expr true e)))
  | Seq c1 c2 => Seq (productTrf c1) (productTrf c2)
- | If b c1 c2 => Seq (Seq (assertEqLeak b)
-                          (assertEqExpr b))
-                     (If ok_get
-                         (If (expr_i false b) (productTrf c1) (productTrf c2))
-                         (Seq (selfComp (If b c1 c2)) (ok_reg okSC_get)))
+ | If b c1 c2 => Seq (assertEqLeakTest b)
+                     (If ok_expr
+                         (If (ren_expr false b) (productTrf c1) (productTrf c2))
+                         (Seq (selfComp lspec (If b c1 c2)) (ok_upd okSC_expr)))
  | While b c1 =>
-    Seq (Seq (assertEqLeak b)
-             (assertEqExpr b))
-        (Seq (While (And ok_get (expr_i false b) )
+    Seq (assertEqLeakTest b)
+        (Seq (While (And ok_expr (ren_expr false b) )
                     (Seq (productTrf c1)
-                         (Seq (assertEqLeak b)
-                              (assertEqExpr b))))
-             (Seq (selfComp (While b c1)) (ok_reg okSC_get)))
+                         (assertEqLeakTest b)))
+             (Seq (selfComp lspec (While b c1)) (ok_upd okSC_expr)))
  end.
 
-Parameter initProduct : cmd ops.
-Parameter assumeEqIn : cmd ops.
-Parameter assumeEqOut : cmd ops.
-Parameter chkOK : cmd ops.
+Definition initProduct: cmd ops :=
+ Assign ok_lvalue (Const _ 1).
 
+Fixpoint assumeVarRestr (v: VarRestr) : cmd ops :=
+ match v with
+ | [::] => Skip _
+ | x::xs => Seq (Assume (Equal (ren_expr false (ValOf (Var _ x))) (ren_expr true (ValOf (Var _ x))))) (assumeVarRestr xs)
+ end.
+
+Variable vIN vOUT: VarRestr.
 
 Definition fullProduct (c: cmd ops) : cmd ops :=
- Seq (Seq initProduct (Seq assumeEqIn (productTrf c)))
-     (Seq assumeEqOut chkOK).
+ Seq (Seq initProduct (Seq (assumeVarRestr vIN) 
+                           (Seq (productTrf c) (assumeVarRestr vOUT))))
+     (Assert ok_expr).
 
-Parameter cmd_i: bool -> cmd ops -> cmd ops.
+Definition trfState0 := mkTrfSt 0 (fun _ => 0).
 
-(*
-Theorem selfComp_A: forall (c:cmd ops) ts1 ts2 (s11 s12 s21 s22: State) l1 l2 l',
- eval_cmd lFun s11 c l1 (Some s21) ->
- eval_cmd lFun s12 c l2 (Some s22) ->
- eval_cmd lFun (joinState ts1 s11 s12) (selfComp c) l' (Some (joinState ts2 s21 s22))
- /\ l1==l2 = true (* ts2[okSC] /\ ok1 = ok2 *).
-Admitted.
+Definition Safe' lspec (c:cmd ops) :=
+ forall st st' l, eval_cmd lspec st c l st' -> st'<>None.
+Definition leakSecure' vIN vOUT c :=
+ forall s1 s2 l1 l2 ss1 ss2,
+   eqstateR vIN s1 s2 ->
+   eval_cmd lspec s1 c l1 ss1 ->
+   eval_cmd lspec s2 c l2 ss2 ->
+   exists s1' s2', ss1 = Some s1' /\ ss2 = Some s2' /\
+   (eqstateR vOUT s1' s2' -> l1 = l2).
 
-Theorem selfComp_B: forall (c:cmd ops) ts1 ts2 (s11 s12 s21 s22: State) l1 l2 l',
- eval_cmd lFun (joinState ts1 s11 s12) (selfComp c) l' (Some (joinState ts2 s21 s22)) ->
- eval_cmd lFun s11 c l1 (Some s21) /\
- eval_cmd lFun s12 c l2 (Some s22) /\
- True (* ts2[okSC] = l1==l2 /\ ok1 = ok2 *).
-Admitted.
-
+Theorem fullProduct_sound: forall c,
+ Safe' lspec (fullProduct c) ->
+ leakSecure' vIN vOUT c.
+Proof.
+rewrite /leakSecure' => c H s1 s2 l1 l2 ss1 ss2 HIN H1 H2.
+move: {H} (H (joinState (s1,s2,trfState0))) => H.
+(* ??? tem interesse ???
+eqstateR vIN s1 s2 ->
+eval_cmd lspec s1 c l1 s1' ->
+eval_cmd lspec s2 c l2 s2' ->
+eval_cmd lspec (joinState (s1,s2,trfState0)) (fullProduct' c) ss
+/\ ss <> None -> s1' <> None /\ s2' <> None.
 *)
+move: ss1 H1 => [s1'|] H1; last first.
+ admit (* H1 -> absurd H 
+pq. eval_cmd lspec s1 c l1 None ->
+    eval_cmd lspec (joinState (s1, s2, trfState0)) (fullProduct c) ll None
+*).
+move: ss2 H2 => [s2'|] H2; last first.
+ admit (* H2 -> absurd H 
+pq. eval_cmd lspec s2 c l2 None ->
+    eval_cmd lspec (joinState (s1, s2, trfState0)) (fullProduct c) ll None
+*).
+exists s1', s2'; split => //.
+split => // HOUT.
+(* 
+ HIN : eqstateR vIN s1 s2
+ H1 : eval_cmd lspec s1 c l1 (Some s1')
+ H2 : eval_cmd lspec s2 c l2 (Some s2')
+ HOUT : eqstateR vOUT s1' s2'
+ =======
+ exists ll s',
+ eval_cmd lspec (joinState (s1, s2, trfState0))
+                (fullProduct' c) ll (Some s')
+ /\ eval_expr s' ok_expr != 0 -> l1=l2
+*)
+admit.
+Qed.
+
+
+Theorem fullProduct_complete: forall c,
+ leakSecure' vIN vOUT c -> 
+ Safe' lspec (fullProduct c).
+Proof.
+rewrite /Safe' /leakSecure' => c H st.
+move => [st'|] l H' => //.
+ (* H' -> !assertOK \/ eval_cmd lspec st (fullProduct' c) l None
+   (1) -> absurd H
+   (2) -> eval_cmd lspec s1 c l1 None \/ eval_cmd lspec s2 c l2 None
+   (3,4) -> absurd H
+ *)
+inversion_clear H'.
+ inversion_clear H1.
+ admit.
+inversion_clear H0; last first.
+ admit (* simple *).
+inversion_clear H2; last first.
+ admit (* simple *).
+inversion_clear H3. 
+ admit (* simple *).
+(* H2 : eval_cmd lspec st0 (productTrf c) l3 ss'
+   ===
+   eval_cmd lspec s1 c l1 ss1 /\
+   eval_cmd lspec s2 c l2 ss2 /\ ss' = Some st' -> ss1 = Some (st'.1.1)...
+*)
+admit.
+Qed.
+
