coq-formalisations/FullProduct/SelfComp.v
@@ -12,87 +12,273 @@ Definition ident := positive.
 
 Open Scope Z_scope.
 
+Definition okSC_idx : Z := (-1).
+Definition clSC_idx : Z := (-2).
+Definition crSC_idx : Z := (-3).
 
-
+Definition okSC (s:trfState) : Z := sc s (-1).
+Definition clSC (s:trfState) : Z := sc s (-2).
+Definition crSC (s:trfState) : Z := sc s (-3).
+Definition leakSC (s:trfState) (i:Z) : Z := sc s i.
 
 Section SCtrf.
 
 Variable ops: opSig.
 
-Variable lFun : LeakFun ops.
+Record LeakSpec :=
+ { lFun :> @LeakFun ops
+ ; preleak: expr ops -> seq (expr ops)
+ ; preleak_ren: forall f e,
+     preleak (ren_expr f e) = map (ren_expr f) (preleak e)
+ ; preleak_prod: forall s1 s2 e,
+     (leak_expr preleak s1 e == leak_expr preleak s2 e)
+     = (leak_expr lFun s1 e == leak_expr lFun s2 e)
+ }.
 
-Definition ok: ident := xH.
-Definition okSC: ident := xO xH.
-Definition cL: ident := xI xH.
-Definition cR: ident := xO (xO xH).
-Definition leakL: ident := xH.
-(* obs: uma alternativa era registar toda a informação SC no array
-    leak[0] = ok
-    leak[1] = countL
-    leak[2] = countR
-    leak[3..] = leakage...
-PARECE BOA IDEIA!!! :-)
-*)
+Variable lspec: LeakSpec.
+
+Definition ok_lvalue: lvalue ops := Var _ xH.
+Definition okSC_lvalue := ArrCell xH (Const ops okSC_idx).
+Definition clSC_lvalue := ArrCell xH (Const ops clSC_idx).
+Definition crSC_lvalue := ArrCell xH (Const ops crSC_idx).
+Definition leakSC_lvalue (e: expr ops) : lvalue ops := ArrCell xH e.
+Definition ok_expr: expr ops := ValOf ok_lvalue.
+Definition okSC_expr: expr ops := ValOf okSC_lvalue.
+Definition clSC_expr: expr ops := ValOf clSC_lvalue.
+Definition crSC_expr: expr ops := ValOf crSC_lvalue.
+Definition leakSC_expr (e: expr ops) : expr ops := ValOf (leakSC_lvalue e).
+
+Definition initSC: cmd ops :=
+ Seq (Assign okSC_lvalue (Const _ 1))
+     (Seq (Assign clSC_lvalue (Const _ 0))
+          (Assign crSC_lvalue (Const _ 0))).
+
+Definition okSC_upd (e: expr ops) : cmd ops :=
+ Assign okSC_lvalue (And okSC_expr e).
+Definition clSC_inc : cmd ops :=
+ Assign clSC_lvalue (Minus clSC_expr (Const _ (-1))).
+Definition crSC_inc : cmd ops :=
+ Assign crSC_lvalue (Minus crSC_expr (Const _ (-1))).
 
 
-Parameter regLeak : expr ops -> cmd ops.
-Parameter chkLeak : expr ops -> cmd ops.
-Parameter initSC: cmd ops.
-Parameter chkSC: cmd ops.
+(** registers the (pre)leakage of an expression *)
 
-Parameter  preleak: expr ops -> seq (expr ops).
-Parameter expr_i: bool -> expr ops -> expr ops.
-Parameter lvalue_i: bool -> lvalue ops -> lvalue ops.
+Definition regVal (e: expr ops) : cmd ops :=
+ Seq (Assign (leakSC_lvalue clSC_expr) e) clSC_inc.
+
+(** checks the (pre)leakage of an expression against registered one *)
+
+Definition chkVal (e: expr ops) : cmd ops :=
+ Seq (okSC_upd (Equal (leakSC_expr crSC_expr) e)) crSC_inc.
 
 Fixpoint procLeak (side:bool) (l: seq (expr ops)) : cmd ops :=
  match l, side with
  | [::], _ => @Skip ops
- | e::es, false => Seq (regLeak e) (procLeak side es)
- | e::es, true => Seq (chkLeak e) (procLeak side es)
+ | e::es, false => Seq (regVal e) (procLeak side es)
+ | e::es, true => Seq (chkVal e) (procLeak side es)
  end.
 
 Fixpoint mirror (side:bool) (c: cmd ops) {struct c} : cmd ops :=
  match c with
  | Skip => @Skip ops
- | Assert e => Assert (expr_i side e)
- | Assume e => Assume (expr_i side e)
- | Assign x e => Seq (Seq (procLeak side (preleak (expr_i side (ValOf x))))
-                          (procLeak side (preleak (expr_i side e))))
-                     (Assign (lvalue_i side x) (expr_i side e))
+ | Assert e => Assert (ren_expr side e)
+ | Assume e => Assume (ren_expr side e)
+ | Assign x e => Seq (Seq (procLeak side (preleak lspec (ren_expr side (ValOf x))))
+                          (procLeak side (preleak lspec (ren_expr side e))))
+                     (Assign (ren_lvalue side x) (ren_expr side e))
  | Seq c1 c2 => Seq (mirror side c1) (mirror side c2)
- | If b c1 c2 => Seq (Seq (procLeak side (preleak (expr_i side b)))
-                          (procLeak side [:: expr_i side b]))
-                     (If (expr_i side b) (mirror side c1) (mirror side c2))
+ | If b c1 c2 => Seq (Seq (procLeak side (preleak lspec (ren_expr side b)))
+                          (procLeak side [:: IsTrue (ren_expr side b)]))
+                     (If (ren_expr side b) (mirror side c1) (mirror side c2))
  | While b c1 =>
-    Seq (Seq (procLeak side (preleak (expr_i side b)))
-             (procLeak side [:: expr_i side b]))
-        (While (expr_i side b) 
+    Seq (Seq (procLeak side (preleak lspec (ren_expr side b)))
+             (procLeak side [:: IsTrue (ren_expr side b)]))
+        (While (ren_expr side b) 
                (Seq (mirror side c1)
-                    (Seq (procLeak side (preleak (expr_i side b)))
-                         (procLeak side [:: expr_i side b]))))
+                    (Seq (procLeak side (preleak lspec (ren_expr side b)))
+                         (procLeak side [:: IsTrue (ren_expr side b)]))))
  end.
                  
 Definition selfComp (c: cmd ops) : cmd ops :=
- (Seq (Seq initSC (Seq (mirror false c) (mirror true c))) chkSC).
+ Seq (Seq initSC (Seq (mirror false c) (mirror true c))) 
+     (okSC_upd (Equal clSC_expr crSC_expr)).
 
-Parameter cmd_i: bool -> cmd ops -> cmd ops.
+Fixpoint matchLeak side (st:trfState) (start:Z) (l: seq Z) :=
+ match l with
+ | [::] => start == (if side then crSC st else clSC st)
+ | (x::xs) => (x==leakSC st start) && (matchLeak side st (start+1) xs)
+ end.
+
+Inductive mirror1_spec : seq Z -> trfState -> trfState -> Prop :=
+ | mirror1_nil: forall st, mirror1_spec [::] st st
+ | mirror1_cons: forall x xs st st',
+     mirror1_spec xs (mkTrfSt (ok st) (upd (upd (leakSC st) (clSC st) x) 
+                                           clSC_idx (clSC st + 1))) st' ->
+     mirror1_spec (x::xs) st st'.
+
+Inductive mirror2_spec : seq Z -> trfState -> trfState -> Prop :=
+ | mirror2_nil: forall st, mirror2_spec [::] st st
+ | mirror2_cons: forall x xs st st',
+     mirror2_spec xs (mkTrfSt (ok st)
+                              (upd (upd (leakSC st) okSC_idx
+                                        (if x==leakSC st crSC_idx
+                                         then okSC st
+                                         else 0))
+                                   crSC_idx (crSC st + 1))) st' ->
+     mirror2_spec (x::xs) st st'.
+
+(*
+mirror1_spec_cat:
+mirror1_spec l1 st1 st2 -> mirror1_spec l2 st2 st3 ->
+mirror1_spec (l1++l2) st1 st3.
+
+procLeak1_spec:
+
+exists ll,
+ eval_cmd lspec (joinState (s1,s2,st))
+   (procLeak false (preleak lspec (ren_expr false e)))
+   ll (joinState (s1,s2,updLeakL st (leak_expr lspec (ren_expr false e))))
+                        ========
 
 
-Theorem selfComp_A: forall (c:cmd ops) ts1 ts2 (s11 s12 s21 s22: State) l1 l2 l',
- eval_cmd lFun s11 c l1 (Some s21) ->
- eval_cmd lFun s12 c l2 (Some s22) ->
- eval_cmd lFun (joinState ts1 s11 s12) (selfComp c) l' (Some (joinState ts2 s21 s22))
- /\ l1==l2 = true (* ts2[okSC] /\ ok1 = ok2 *).
+
+Fixpoint updLeakL st l :=
+ match l with
+ | [::] => st
+ | (x::xs) =>
+    updLeakL (mkTrfSt (ok st) (upd (upd (leakSC st) (clSC st) x) 
+                                   clSC_idx (clSC st + 1)))
+             xs
+ end.
+*)
+
+Lemma mirror1_sound: forall c s1 s2 st l1 s1',
+ eval_cmd lspec s1 c l1 (Some s1') ->
+ exists ll st',
+  eval_cmd lspec (joinState (s1,s2,st)) (mirror false c) ll 
+                 (Some (joinState (s1',s2,st')))
+  /\ mirror1_spec l1 st st'.
+Proof.
+move => c s1 s2 st l1 s1' /eval_cmd_feval [n H].
+elim: n s1 s1' l1 c H => //.
+move => n IH s1 s1' l1 [|e|e|x e|c1 c2|b c1 c2|b c] /=.
+- (* Skip *)
+  admit.
+- (* Assume *)
+  admit.
+- (* Assert *)
+  admit.
+- (* Assign *)
+  move => [<- <-].
+  admit.
+- (* Seq *)
+  admit.
+- (* If *)
+  admit.
+- (* While *)
+  admit.
+Qed.
+
+Lemma mirror1_complete: forall c s1 s2 st l1 ll s',
+ eval_cmd lspec (joinState (s1,s2,st)) (mirror false c) ll 
+                (Some s') ->
+ mirror1_spec l1 st (splitState s').2 ->
+ eval_cmd lspec s1 c l1 (Some (splitState s').1.1).
+Proof.
+admit (*
+move => c s1 s2 st l1 s1' /eval_cmd_feval [n H].
+elim: n s1 s1' l1 c H => //.
+move => n IH s1 s1' l1 [|e|e|x e|c1 c2|b c1 c2|b c] /=.
+- (* Skip *)
+  admit.
+- (* Assume *)
+  admit.
+- (* Assert *)
+  admit.
+- (* Assign *)
+  move => [<- <-].
+  admit.
+- (* Seq *)
+  admit.
+- (* If *)
+  admit.
+- (* While *)
+  admit.
+*).
+Qed.
+
+Lemma mirror2_sound: forall c s1 s2 st l2 s2',
+ eval_cmd lspec s2 c l2 (Some s2') ->
+ exists ll st',
+  eval_cmd lspec (joinState (s1,s2,st)) (mirror true c) ll 
+                 (Some (joinState (s1,s2',st')))
+  /\ mirror2_spec l2 st st'.
+Proof.
+move => c s1 s2 st l2 s2' /eval_cmd_feval [n H].
+elim: n s2 s2' l2 c H => //.
+move => n IH s2 s2' l2 [|e|e|x e|c1 c2|b c1 c2|b c] /=.
+- (* Skip *)
+  admit.
+- (* Assume *)
+  admit.
+- (* Assert *)
+  admit.
+- (* Assign *)
+  move => [<- <-].
+  admit.
+- (* Seq *)
+  admit.
+- (* If *)
+  admit.
+- (* While *)
+  admit.
+Qed.
+
+Lemma mirror2_complete: forall c s1 s2 st l2 ll s',
+ eval_cmd lspec (joinState (s1,s2,st)) (mirror true c) ll 
+                (Some s') ->
+ mirror2_spec l2 st (splitState s').2 ->
+ eval_cmd lspec s2 c l2 (Some (splitState s').1.2).
+Proof.
+admit (*
+move => c s1 s2 st l1 s1' /eval_cmd_feval [n H].
+elim: n s1 s1' l1 c H => //.
+move => n IH s1 s1' l1 [|e|e|x e|c1 c2|b c1 c2|b c] /=.
+- (* Skip *)
+  admit.
+- (* Assume *)
+  admit.
+- (* Assert *)
+  admit.
+- (* Assign *)
+  move => [<- <-].
+  admit.
+- (* Seq *)
+  admit.
+- (* If *)
+  admit.
+- (* While *)
+  admit.
+*).
+Qed.
+
+Theorem selfComp_sound:
+ forall (c:cmd ops) ts ts' (s1 s1' s2 s2' s': State) l1 l2 l',
+ eval_cmd (lFun lspec) s1 c l1 (Some s1') ->
+ eval_cmd (lFun lspec) s2 c l2 (Some s2') ->
+ eval_cmd (lFun lspec) (joinState (s1,s2,ts)) (selfComp c) l'
+                       (Some (joinState (s1',s2',ts')))
+ /\ l1==l2 = (eval_expr (joinState (s1',s2',ts')) okSC_expr != 0).
 Admitted.
 
-Theorem selfComp_B: forall (c:cmd ops) ts1 ts2 (s11 s12 s21 s22: State) l1 l2 l',
- eval_cmd lFun (joinState ts1 s11 s12) (selfComp c) l' (Some (joinState ts2 s21 s22)) ->
- eval_cmd lFun s11 c l1 (Some s21) /\
- eval_cmd lFun s12 c l2 (Some s22) /\
- True (* ts2[okSC] = l1==l2 /\ ok1 = ok2 *).
+Theorem selfComp_complete:
+ forall (c:cmd ops) ts1 (s11 s12 s2: State) l1 l2 l',
+ eval_cmd (lFun lspec) (joinState (s11,s12,ts1)) (selfComp c) l'
+                       (Some s2) ->
+ eval_cmd (lFun lspec) s11 c l1 (Some (splitState s2).1.1) /\
+ eval_cmd (lFun lspec) s12 c l2 (Some (splitState s2).1.2) /\
+ l1==l2 = (eval_expr s2 okSC_expr != 0).
 Admitted.
-
-
 
 End SCtrf.
 
